veric/null_extension.v
@@ -38,8 +38,9 @@ Section NullExtension.
  
  Program Definition null_extension := Extension.Make 
   (fun i:nat => Genv.t (const fT i) (const vT i))
-  csemT cores csig csig handled proj_core active _ proj_zint proj_zext zmult 
+  csemT cores csig csig handled 1 proj_core _ active _ proj_zint proj_zext zmult 
   _ _ _ _ _ _.
+ Next Obligation. if_tac; auto. rewrite H0 in H. elimtype False; omega. Qed.
  Next Obligation. if_tac; exists s; auto. elimtype False; apply H; auto. Qed.
  Next Obligation. inversion H; subst; eapply at_external_handled; eauto. Qed.
  Next Obligation. 
@@ -284,7 +285,7 @@ Section NullExtensionCompilable.
  Variable core_simulation: Forward_simulation_inject dS dT csemS csemT 
    geS geT entry_points core_data match_state core_ord.
  Variable core_simulationsRG: forall i:nat, 
-   RelyGuaranteeSimulation.Sig csemS csemT match_state.
+   RelyGuaranteeSimulation.Sig csemS csemT geS match_state.
  Variable threads_max: nat.
  Variable threads_max_nonzero: (O < threads_max)%nat. (*Required by defn. of core_ords*)
 
@@ -299,10 +300,11 @@ Section NullExtensionCompilable.
  Proof.
  (*SOLVED BY econstructor; eauto.  WE'LL USE THE PROVIDED LEMMAS INSTEAD.*)
  intros H1 H2 H3.
+ set (R := fun (_:meminj) (_:cS) (_:mem) (_:cT) (_:mem) => True).
  destruct (@ExtensionCompilability
    _ _ _ _ _ _ _ _ _ _ _ _ _ _ _ 
    csemS csemT csemS csemT csig csig handled 
-   geS geT geS geT E_S E_T entry_points core_data match_state core_ord threads_max)
+   geS geT geS geT E_S E_T entry_points core_data match_state core_ord threads_max R)
   as [LEM].
  apply LEM; auto.
  solve[intros i; unfold const; apply genvs_domain_eq_refl; auto].
@@ -312,12 +314,12 @@ Section NullExtensionCompilable.
  unfold E_T, const.
  solve[apply (null_core_compatible geT csig at_external_handledT H2)].
 
- constructor.
- solve[intros; eapply match_state_runnable; eauto].
+ constructor; try solve[intros; unfold R; auto].
+(* solve[intros; eapply match_state_runnable; eauto].*)
 
  intros until j; intros H4 H5 H6 H7 H8 H9 H10 H11 H12 H13 H14 H15.
  destruct core_simulation; unfold const; simpl.
- destruct H10 as [? MATCH].
+ destruct H10 as [? [? MATCH]].
  specialize (MATCH O s1).
  spec MATCH; auto.
  destruct MATCH as [_s2 [PROJ MATCH]].
@@ -329,13 +331,14 @@ Section NullExtensionCompilable.
  split3; auto.
  split; auto.
  split; auto.
+ split; auto.
  intros i _s1'; simpl; unfold proj_core; intros PROJ.
  if_tac in PROJ; try congruence.
  inv PROJ.
  solve[exists s2'; auto].
- destruct H17.
+ destruct H18.
  solve[left; auto].
- destruct H17 as [A B].
+ destruct H18 as [A B].
  right; split; auto.
  unfold CompilabilityInvariant.core_ords.
  exists O. 
@@ -350,7 +353,10 @@ Section NullExtensionCompilable.
  intros; destruct core_simulation.
  destruct (core_initial0 v1 v2 sig H vals1 s1 m1 j vals2 m2 H0 H4 H5 H6) 
   as [cd [s2 [H7 H8]]].
- exists (fun _ => cd); exists s2; split; auto. split; auto.
+ exists (fun _ => cd); exists s2; split; auto. 
+ split; auto.
+ solve[unfold R; auto].
+ split; auto.
  intros i c1 H9; exists s2; split; auto.
  simpl in H9; unfold proj_core in H9|-*; if_tac in H9; try congruence.
  solve[inv H9; split; auto].
@@ -360,7 +366,7 @@ Section NullExtensionCompilable.
 
  intros until v1; intros MATCH12 HALT.
  unfold CompilabilityInvariant.match_states, const in MATCH12.
- destruct MATCH12 as [? MATCH12].
+ destruct MATCH12 as [? [? MATCH12]].
  specialize (MATCH12 O c1).
  spec MATCH12; auto.
  destruct MATCH12 as [c2' [PROJ MATCH12]].
